examples, tests, etc

src/Model/Bernoulli.dfy
@@ -7,12 +7,14 @@ include "Monad.dfy"
 include "RandomNumberGenerator.dfy"
 include "Independence.dfy"
 include "Uniform.dfy"
+include "MeasureTheory.dfy"
 
 module Bernoulli {
   import opened Monad
   import opened RandomNumberGenerator
   import opened Independence
   import opened Uniform
+  import opened MeasureTheory
 
   /************
    Definitions  
@@ -39,9 +41,11 @@ module Bernoulli {
   }  
 
   // Footnote 5, p. 82
-  function ProbBernoulliRational(m: nat, n: nat): Hurd<bool> 
+  function ProbBernoulliRational(m: nat, n: nat): (f: Hurd<bool>)
     requires n != 0
     requires m <= n
+    ensures forall s :: f(s).0 == (ProbUniform(n)(s).0 < m)
+    ensures forall s :: f(s).1 == ProbUniform(n)(s).1
   {
     Bind(ProbUniform(n), (k: nat) => Return(k < m))
   }
@@ -71,7 +75,7 @@ module Bernoulli {
     IndepFnIsCompositional(f, g);
   }
 
-  lemma BernoulliRationalCorrectness(m: nat, n: nat)
+  lemma {:vcs_split_on_every_assert} BernoulliRationalCorrectness(m: nat, n: nat)
     requires n != 0
     requires m <= n
     ensures
@@ -80,41 +84,59 @@ module Bernoulli {
       && mu(e) == m as real / n as real
   {
     var e := iset s | ProbBernoulliRational(m, n)(s).0;
-    var e1 := iset s | ProbUniform(n)(s).0 == m-1;
 
-    assert m - 1 <= m <= n;
-    var e2 := iset s | ProbBernoulliRational(m-1, n)(s).0;
+    if m == 0 {
+      assert e == iset{};
+      RNGHasMeasure();
+      assert mu(e) == 0.0 by {
+        assert IsPositive(event_space, mu);
+      }
+    } else {
+      var e1 := iset s | ProbUniform(n)(s).0 == m-1;
+      var e2 := (iset s {:trigger ProbUniform(n)(s).0} | ProbBernoulliRational(m-1, n)(s).0);
 
-    calc {
-      e;
-      iset s | ProbUniform(n)(s).0 < m;
-      iset s | ProbUniform(n)(s).0 == m-1 || ProbUniform(n)(s).0 < m-1;
-      (iset s | ProbUniform(n)(s).0 == m-1) + (iset s | ProbUniform(n)(s).0 < m-1);
+      assert (iset s | ProbUniform(n)(s).0 < m-1) == e2 by {
+        assert (iset s | ProbUniform(n)(s).0 < m-1) == (iset s {:trigger ProbUniform(n)(s).0} | ProbBernoulliRational(m-1, n)(s).0) by {
+          forall s ensures ProbUniform(n)(s).0 < m-1 <==> ProbBernoulliRational(m-1, n)(s).0 {
+            assert ProbUniform(n)(s).0 < m-1 <==> ProbBernoulliRational(m-1, n)(s).0;
+          }
+        }
+      }
+
+      calc {
+        e;
+        iset s | ProbUniform(n)(s).0 < m;
+        iset s | ProbUniform(n)(s).0 == m-1 || ProbUniform(n)(s).0 < m-1;
+        (iset s | ProbUniform(n)(s).0 == m-1) + (iset s | ProbUniform(n)(s).0 < m-1);
+        e1 + e2;
+      }
+      
+      assert e1 in event_space && mu(e1) == 1.0 / (n as real) by {
+        UniformFullCorrectness(n, m-1);
+      }
+
+      assert e2 in event_space && mu(e2) == (m - 1) as real / n as real by {
+        BernoulliRationalCorrectness(m-1, n);
+      }
+
+      assume {:axiom} false;
+
+      assert e in event_space by {
+        RNGHasMeasure();
+        BinaryUnion(event_space, sample_space, e1, e2);
+      }
+
+      calc {
+        mu(e);
+        mu(e1 + e2);
+        { assert e1 * e2 == iset{}; }
+        mu(e1) + mu(e2);
+        (1.0 / (n as real)) + ((m-1) as real / n as real);
+        (1.0 + ((m-1) as real)) / n as real;
+        (1.0 + (m as real) - 1.0) / n as real;
+        m as real / n as real;
+      } 
     }
-
-    assume {:axiom} false;
-
-/*     assert (iset s | ProbUniform(n)(s).0 == m-1) == e1;
-    assert (iset s | ProbUniform(n)(s).0 < m-1) == e2;
-    
-    assert mu(e1) == 1.0 / (n as real) by {
-      UniformFullCorrectness(n, m-1);
-    }
-
-    assert mu(e2) == (m - 1) as real / n as real by {
-      BernoulliRationalCorrectness(m-1, n);
-    }
-
-    calc {
-      mu(e);
-      mu(e1 + e2);
-      { assert e1 * e2 == iset{}; }
-      mu(e1) + mu(e2);
-      (1.0 / (n as real)) + ((m-1) as real / n as real);
-      (1.0 + ((m-1) as real)) / n as real;
-      (1.0 + (m as real) - 1.0) / n as real;
-      m as real / n as real;
-    }  */
   }
 
   lemma {:axiom} ProbBernoulliIsIndepFn(p: Probability)
