tests/Tests.dfy
@@ -94,6 +94,22 @@
     testEmpiricalIsWithin3SigmaOfTrueMean(n, sum as real, (1.0 - 0.5) / 0.5, (1.0 - 0.5) / (0.5 * 0.5), "mean");
   }
 
+  method {:test} TestBernoulliRational()
+    decreases *
+  {
+    var n := 1000000;
+    var r := new DRandom();
+
+    var t := 0;
+    for i := 0 to n {
+      var b := r.BernoulliRational(1, 5);
+      if b {
+        t := t + 1;
+      }
+    }
+    testBernoulliIsWithin3SigmaOfTrueMean(n, t as real, 0.2, "p(true)");
+  }
+
   method {:test} TestBernoulli()
     decreases *
   {
